src/ADTRefinement/GeneralBuildADTRefinements.v
@@ -93,8 +93,8 @@ Section BuildADTRefinements.
             adt''
     :
       (let H := consBody newDef in refineConstructor eq (consBody (ith consDefs idx)) H)
-    -> FullySharpenedUnderDelegates RCods HRCodsRefl (ADTReplaceConsDef consDefs methDefs idx newDef) adt''
-    -> FullySharpenedUnderDelegates RCods HRCodsRefl (BuildADT consDefs methDefs) adt''.
+    -> FullySharpenedUnderDelegates RCods (ADTReplaceConsDef consDefs methDefs idx newDef) adt''
+    -> FullySharpenedUnderDelegates RCods (BuildADT consDefs methDefs) adt''.
   Proof.
     intros; eapply FullySharpenStep; eauto; try exact X.
     eapply refineADT_BuildADT_ReplaceConstructor with (AbsR_mono := eq) (AbsR_anti := eq);
@@ -369,7 +369,6 @@ Lemma refineADT_BuildADT_ReplaceConstructor_sigma
   Definition Notation_Friendly_FullySharpened_BuildMostlySharpenedcADT
              (RepT : Type)
              RCods
-             {HRCodsRefl : forall A, Reflexive (RCods A)}
              {n n'}
              {consSigs : Vector.t consSig n}
              {methSigs : Vector.t methSig n'}
@@ -454,7 +453,7 @@ Lemma refineADT_BuildADT_ReplaceConstructor_sigma
                                              (methCod (Vector.nth methSigs idx))
                                              (getMethDef methDefs idx)
                                              (LiftcMethod (ith (cMethods DelegateReps DelegateImpls) idx))))
-  : FullySharpenedUnderDelegates RCods HRCodsRefl (BuildADT consDefs methDefs)
+  : FullySharpenedUnderDelegates RCods (BuildADT consDefs methDefs)
                                  {|
                                    Sharpened_DelegateSigs := DelegateSigs;
                                    Sharpened_Implementation := Notation_Friendly_BuildMostlySharpenedcADT
@@ -462,7 +461,7 @@ Lemma refineADT_BuildADT_ReplaceConstructor_sigma
                                    Sharpened_DelegateSpecs := DelegateSpecs |}.
   Proof.
     intros * DelegateReps DelegateImpls DelegateImplRefinesSpec.
-    eapply (@refinesADT RCods _ _ (BuildADT consDefs methDefs)
+    eapply (@refinesADT RCods _ (BuildADT consDefs methDefs)
                         (LiftcADT (existT _ (rep DelegateReps)
                                           {| pcConstructors := _;
                                              pcMethods := _|}))
@@ -598,7 +597,6 @@ Lemma refineADT_BuildADT_ReplaceConstructor_sigma
              (RepT : Type)
              {m n n'}
              RCods
-             {HRCodsRefl : forall A, Reflexive (RCods A)}
              (consSigs : Vector.t consSig n)
              (methSigs : Vector.t methSig n')
              (consDefs : ilist consSigs)
@@ -689,7 +687,7 @@ Lemma refineADT_BuildADT_ReplaceConstructor_sigma
                                              (getMethDef methDefs idx)
                                              (LiftcMethod (ith (cMethods DelegateReps DelegateImpls) idx))))
   : FullySharpenedUnderDelegates
-      RCods HRCodsRefl
+      RCods
       (BuildADT consDefs methDefs)
       {|
         Sharpened_DelegateSigs := DelegateSigs;
